DynamoDbEncryption/dafny/DynamoDbEncryption/Model/DynamoDbEncryption.smithy
@@ -713,11 +713,12 @@ structure SingleKeyStore {
   @required
   @javadoc("The Beacon Key ID.")
   keyId : String,
-  @javadoc("How long (in seconds) the beacon key material is cached locally before it is re-retrieved from DynamoDB and re-authed with AWS KMS. Provide only one of cacheTTL or cache.")
+  @required
+  @javadoc("How long (in seconds) the beacon key material is cached locally before it is re-retrieved from DynamoDB and re-authed with AWS KMS.")
   cacheTTL: Integer,
-  @documentation("Provide the Shared Cache for Searchable Encryption. Provide only one of cacheTTL or cache.")
+  @documentation("Provide the Shared Cache for Searchable Encryption.")
   cache : CacheType,
-  @documentation("Partition ID to share DynamoDB Interceptors. TODO: Update description")
+  @documentation("Partition ID to distinguish Beacon Key Sources writing to a cache. If the Partition ID is the same for two Beacon Key Sources, they can share the same cache entries in the cache.")
   partitionId: String
 }
 
@@ -738,7 +739,7 @@ structure MultiKeyStore {
   cacheTTL: Integer,
   @javadoc("Which type of local cache to use.")
   cache : CacheType,
-  @documentation("Partition ID to share DynamoDB Interceptors. TODO: Update description")
+  @documentation("Partition ID to distinguish Beacon Key Sources writing to a cache. If the Partition ID is the same for two Beacon Key Sources, they can share the same cache entries in the cache.")
   partitionId: String
 }
 
